pulse/lib/steel/pulse/Pulse.Typing.Combinators.fst
@@ -270,3 +270,31 @@ let apply_frame (#g:env)
     let st_equiv = ST_VPropEquiv g c' c'' x pre_typing res_typing post_typing ve (VE_Refl _ _) in
     let t_typing = T_Equiv _ _ _ _ t_typing st_equiv in
     (| c'', t_typing |)
+
+let return_in_ctxt (g:env) (y:var) (u:universe) (ty:term) (ctxt:vprop)
+  (ty_typing:universe_of g ty u)
+  (post_hint0:post_hint_opt g { Some? post_hint0 /\ x_t_ctxt_match_post_hint g post_hint0 y ty ctxt})
+
+  : Pure (st_typing_in_ctxt g ctxt post_hint0)
+         (requires lookup g y == Some ty)
+         (ensures fun _ -> True) =
+
+  let Some post_hint = post_hint0 in
+
+  let x = fresh g in
+  assume (~ (x `Set.mem` freevars post_hint.post));
+  let d = T_Return g STT false u ty (null_var y) post_hint.post x ty_typing
+    (magic ())  // that null_var y is well typed at ty in g, we know since lookup g y == Some ty
+    (magic ())  // typing of (open post x) in (g, x) ... post_hint is well-typed, so should get
+  in
+  let t = wr (Tm_Return {ctag=STT;insert_eq=false;term=null_var y}) in
+  let c = comp_return STT false u ty (null_var y) post_hint.post x in
+  let d : st_typing g t c = d in
+
+  let _ :squash (comp_pre c == ctxt /\ comp_post_matches_hint c (Some post_hint)) =
+    match post_hint0 with
+    | Some post_hint ->
+      // this u should follow from equality of t
+      assume (comp_u c == post_hint.u) in
+
+  (| _, _, d |)
